cava/cava/Cava/Arrow/CavaArrow.v
@@ -26,7 +26,6 @@ From Cava Require Export Arrow.ArrowKind.
 Local Open Scope category_scope.
 Local Open Scope arrow_scope.
 
-
 (* Class CircuitLaws `(A: Arrow, ! ArrowCopy A, ! ArrowSwap A, ! ArrowDrop A) := {
   cancelr_unit_uncancelr {x}: @cancelr x >>> uncancelr =M= id;
   cancell_unit_uncancell {x}: @cancell _ _ A x >>> uncancell =M= id;
@@ -51,131 +50,156 @@ Local Open Scope arrow_scope.
 }. *)
 
 (* Cava *)
-Notation "[ x ~~> .. ~~> y ~~> z ]" := (morphism (Tuple x .. (Tuple y Unit) ..) z) : arrow_scope.
-Class Cava := {
-  cava_cat :> Category Kind;
-  cava_arrow :> Arrow Kind cava_cat Unit Tuple;
-  cava_arrow_stkc :> ArrowSTKC cava_arrow;
-  cava_arrow_loop :> ArrowLoop cava_arrow;
 
-  vec_index n := Vector Bit (Nat.log2_up n);
+Local Notation "[ x ~~~> .. ~~~> y ]" := (Tuple x .. (Tuple y Unit) ..).
 
-  constant : bool -> (Unit ~> Bit);
-  constant_bitvec n: N -> (Unit ~> Vector Bit n);
+Notation vec_index n := (Vector Bit (Nat.log2_up n)).
 
-  mk_module i o: string -> (i~>o) -> (i~>o);
+Inductive CircuitPrimitive :=
+  | constant (b: bool)
+  | constant_bitvec (n: nat) (v: N)
+  | delay_gate (o: Kind)
+  | not_gate 
+  | buf_gate
+  | uncons (n: nat) (o: Kind)
+  | unsnoc (n: nat) (o: Kind)
+  | slice (n: nat) (x y: nat) (o: Kind) 
+  | split (n m: nat) (o: Kind) 
+  | empty_vec (o: Kind)
+  | lut (n: nat) (f: bool^^n --> bool)
 
-  not_gate:  [ Bit ~~> Bit ];
-  and_gate:  [ Bit ~~> Bit ~~> Bit];
-  nand_gate: [ Bit ~~> Bit ~~> Bit];
-  or_gate:   [ Bit ~~> Bit ~~> Bit];
-  nor_gate:  [ Bit ~~> Bit ~~> Bit];
-  xor_gate:  [ Bit ~~> Bit ~~> Bit];
-  xnor_gate: [ Bit ~~> Bit ~~> Bit];
-  buf_gate:  [ Bit         ~~> Bit];
+  | and_gate  
+  | nand_gate 
+  | or_gate   
+  | nor_gate
+  | xor_gate
+  | xnor_gate 
+  | xorcy
 
-  delay_gate {o} : [ o ~~> o ];
+  | muxcy
+  | unsigned_add (a b c: nat)
+  | unsigned_sub (a: nat)
+  | index (n: nat) (o: Kind)
+  | cons (n: nat) (o: Kind)
+  | snoc (n: nat) (o: Kind)
+  | concat (n m: nat) (o: Kind).
 
-  xorcy:     [ Bit ~~> Bit ~~> Bit ];
-  muxcy:     [ Bit ~~> (Bit ** Bit) ~~> Bit ];
-  
-  unsigned_add a b c: [ Vector Bit a ~~> Vector Bit b ~~> Vector Bit c ];
-  unsigned_sub a: [ Vector Bit a ~~> Vector Bit a ~~> Vector Bit a ];
+Fixpoint primitive_input (op: CircuitPrimitive): Kind :=
+  match op with
+  | constant v => Unit
+  | constant_bitvec n v => Unit
+  | delay_gate o => Tuple o Unit
+  | not_gate => Tuple Bit Unit
+  | buf_gate => Tuple Bit Unit
+  | uncons n o => Tuple (Vector o (S n)) Unit
+  | unsnoc n o => Tuple (Vector o (S n)) Unit
+  | slice n x y o => Tuple (Vector o n) Unit
+  | split n m o => Tuple (Vector o (n+m)) Unit
+  | empty_vec o => Unit
+  | lut n f => Tuple (Vector Bit n) Unit 
 
-  lut n: (bool^^n --> bool) -> [Vector Bit n ~~> Bit];
+  | muxcy => [ Bit ~~~> Tuple Bit Bit ]
+  | unsigned_add a b c => [ Vector Bit a ~~~> Vector Bit b ]
+  | unsigned_sub a => [ Vector Bit a ~~~> Vector Bit a ]
+  | index n o => [ Vector o n ~~~> vec_index n ]
+  | cons n o => [ o ~~~> Vector o n ]
+  | snoc n o => [ Vector o n ~~~> o ]
+  | concat n m o => [ Vector o n ~~~> Vector o m ]
 
-  empty_vec o: u ~> Vector o 0;
-  index n o: [Vector o n ~~> vec_index n ~~> o];
-  cons n o: [o ~~> Vector o n ~~> Vector o (S n)];
-  snoc n o: [Vector o n ~~> o ~~> Vector o (S n)];
-  uncons n o: [Vector o (S n) ~~> o ** Vector o n];
-  unsnoc n o: [Vector o (S n) ~~> Vector o n ** o];
-  concat n m o: [Vector o n ~~> Vector o m ~~> Vector o (n + m)];
-  split n m o: [Vector o (n+m) ~~> Vector o n ** Vector o m];
-  (* slice n x y where x >= y, x is inclusive 
-  So, somevec[1:0] is the vector [vec[0],vec[1]] : Vector 2 _ *)
-  slice n x y o: x < n -> y <= x -> [Vector o n ~~> Vector o (x - y + 1)];
+  | _ => [ Bit ~~~> Bit ]
+  end.
+
+Fixpoint primitive_output (op: CircuitPrimitive): Kind :=
+  match op with
+  | constant v => Bit
+  | constant_bitvec n v => Vector Bit n
+  | delay_gate o => o
+  | not_gate => Bit
+  | buf_gate => Bit
+  | uncons n o => Tuple o (Vector o n)
+  | unsnoc n o => Tuple (Vector o n) o
+  | slice n x y o => Vector o (x - y + 1)
+  | split n m o => Tuple (Vector o n) (Vector o m)
+  | empty_vec o => Vector o 0
+  | lut n f => Bit
+
+  | muxcy => Bit
+  | unsigned_add a b c => Vector Bit c 
+  | unsigned_sub a => Vector Bit a
+  | index n o => o
+  | cons n o => Vector o (S n)
+  | snoc n o => Vector o (S n)
+  | concat n m o => Vector o (n + m)
+
+  | _ => Bit
+  end.
+
+Notation arrow_input x := (arrow_input (object:=Kind) (unit:=Unit) (product:=Tuple) x).
+Notation arrow_output x := (arrow_output (object:=Kind) (unit:=Unit) (product:=Tuple) x).
+
+(* Single clock circuit *)
+Inductive Circuit: Kind -> Kind -> Type := 
+  | Structural: forall (x: ArrowStructure), Circuit (arrow_input x) (arrow_output x)
+  | Primitive: forall (x: CircuitPrimitive), Circuit (primitive_input x) (primitive_output x)
+
+  (* contains subcircuits *)
+  | Composition: forall x y z, Circuit x y -> Circuit y z -> Circuit x z
+  | First: forall x y z, Circuit x y -> Circuit (Tuple x z) (Tuple y z)
+  | Second: forall x y z, Circuit x y -> Circuit (Tuple z x) (Tuple z y)
+  | Loopr: forall x y z, Circuit (Tuple x z) (Tuple y z) -> Circuit x y
+  | Loopl: forall x y z, Circuit (Tuple z x) (Tuple z y) -> Circuit x y
+  .
+
+(* Notation "[ x ~~> .. ~~> y ~~> z ]" := (morphism (Tuple x .. (Tuple y Unit) ..) z) : arrow_scope. *)
+Notation "[ x ~~> .. ~~> y ~~> z ]" := (Circuit (Tuple x .. (Tuple y Unit) ..) z) : arrow_scope.
+
+Instance CircuitCat : Category Kind := {
+  morphism X Y := Circuit X Y;
+  id X := Structural (Id X);
+  compose X Y Z f g := Composition X Y Z g f;
 }.
 
-Coercion cava_cat: Cava >-> Category.
-Coercion cava_arrow: Cava >-> Arrow.
-Coercion cava_arrow_stkc: Cava >-> ArrowSTKC.
-Coercion cava_arrow_loop: Cava >-> ArrowLoop.
+Instance CircuitArrow : Arrow Kind CircuitCat Unit Tuple := {
+  first  f := First f;
+  second f := Second f;
+  assoc   x y z := Structural (Assoc x y z);
+  unassoc x y z := Structural (Unassoc x y z);
+  cancelr  x := Structural (Cancelr x);
+  cancell  x := Structural (Cancell x);
+  uncancell x := Structural (Uncancell x);
+  uncancelr x := Structural (Uncancelr x);
+}.
 
-Declare Scope cava_scope.
-Bind Scope cava_scope with Cava.
-Delimit Scope cava_scope with cava.
-
-Open Scope cava_scope.
+Instance CircuitArrowDrop : ArrowDrop CircuitArrow := { drop _ := Structural (Drop _); }.
+Instance CircuitArrowSwap : ArrowSwap CircuitArrow := { swap _ _ := Structural (Swap _ _); }.
+Instance CircuitArrowCopy : ArrowCopy CircuitArrow := { copy _ := Structural (Copy _); }.
+Instance CircuitArrowLoop : ArrowLoop CircuitArrow := { loopl := Loopl; loopr := Loopr; }.
+Instance CircuitArrowSTKC : ArrowSTKC CircuitArrow := { }.
 
 Ltac match_primitive X :=
   match X with 
-  | (Category.id) => idtac
-
-  | (first _) => idtac
-  | (second _) => idtac
-  | (cancelr) => idtac
-  | (cancell) => idtac
-  | (uncancelr) => idtac
-  | (uncancell) => idtac
-  | (assoc) => idtac
-  | (unassoc) => idtac
-
-  | (CavaArrow.constant _) => idtac
-  | (CavaArrow.constant_bitvec _ _) => idtac
-  | (CavaArrow.mk_module _ _) => idtac
-
-  | (CavaArrow.not_gate) => idtac
-  | (CavaArrow.and_gate) => idtac
-  | (CavaArrow.nand_gate) => idtac
-  | (CavaArrow.or_gate) => idtac
-  | (CavaArrow.nor_gate) => idtac
-  | (CavaArrow.xor_gate) => idtac
-  | (CavaArrow.xnor_gate) => idtac
-  | (CavaArrow.buf_gate) => idtac
-
-  | (CavaArrow.delay_gate _) => idtac
-
-  | (CavaArrow.xorcy) => idtac
-  | (CavaArrow.muxcy) => idtac
-
-  | (CavaArrow.unsigned_add _ _ _) => idtac
-
-  | (CavaArrow.lut _) => idtac
-
-  | (CavaArrow.empty_vec _) => idtac
-  | (CavaArrow.index _ _) => idtac
-
-  | (CavaArrow.cons _ _) => idtac
-  | (CavaArrow.snoc _ _) => idtac
-  | (CavaArrow.uncons _ _) => idtac
-  | (CavaArrow.unsnoc _ _) => idtac
-  | (CavaArrow.concat _ _ _) => idtac
-  | (CavaArrow.split _ _ _ _) => idtac
-  | (CavaArrow.slice _ _ _ _ _ _) => idtac
+  | (Circuit _ _ _) => idtac
   end.
 
 Ltac match_compose X :=
   match X with 
-  | (Category.compose ?Y ?Z) =>
-    (match_primitive Y + match_compose Y); 
-    (match_primitive Z + match_compose Z)
+  | (Composition _ _ ?Y ?Z) => idtac
   end.
 
-Definition high {_: Cava}: Unit ~> Bit := constant true.
-Definition low {_: Cava}: Unit ~> Bit := constant false.
+Definition high : Unit ~> Bit := Primitive (constant true).
+Definition low : Unit ~> Bit := Primitive (constant false).
 
-Fixpoint insert_rightmost_tt `{Cava} (ty: Kind): ty ~> (insert_rightmost_unit ty).
+Fixpoint insert_rightmost_tt (ty: Kind): ty ~> (insert_rightmost_unit ty).
 Proof.
   intros.
   destruct ty.
-  exact (second (insert_rightmost_tt _ ty2)).
+  exact (second (insert_rightmost_tt ty2)).
   exact id.
   exact uncancelr.
   exact uncancelr.
 Defined.
 
-Fixpoint insert_rightmost_tt1 `{Cava} (ty: Kind): (remove_rightmost_unit ty) ~> ty.
+Fixpoint insert_rightmost_tt1 (ty: Kind): (remove_rightmost_unit ty) ~> ty.
 Proof.
   refine (
   Fix arg_length_order_wf (fun ty => (remove_rightmost_unit ty) ~> ty )
@@ -192,7 +216,7 @@ Proof.
   auto.
 Defined.
 
-Fixpoint remove_rightmost_tt `{Cava} (ty: Kind): ty ~> (remove_rightmost_unit ty).
+Fixpoint remove_rightmost_tt (ty: Kind): ty ~> (remove_rightmost_unit ty).
   refine (Fix arg_length_order_wf (fun ty => ty ~> (remove_rightmost_unit ty))
     (fun (ty:Kind)
       (remove_rightmost_tt': forall ty', arg_length_order ty' ty -> ty' ~> (remove_rightmost_unit ty')) =>
