cava/cava/Cava/Arrow/CavaNotation.v
@@ -29,7 +29,7 @@ Delimit Scope kappa_scope with kappa.
 
 Module KappaNotation.
   Notation "<[ e ]>" := (
-    fun (cava: Cava) => Closure_conversion (arrow:=cava) (fun var => e%kappa)
+    Closure_conversion (arrow:=CircuitArrow) (fun var => e%kappa)
    ) (at level 1, e custom expr at level 1).
 
   (* Notation "<[ e ]>" := (e%kappa) (at level 1, e custom expr at level 1). *)
@@ -58,8 +58,8 @@ Module KappaNotation.
 
   (* Escaping *)
 
-  Notation "! x" := (Morph (x _))(in custom expr at level 2, x global) : kappa_scope.
-  Notation "!( x )" := (Morph (x _)) (in custom expr, x constr) : kappa_scope.
+  Notation "! x" := (Morph (x ))(in custom expr at level 2, x global) : kappa_scope.
+  Notation "!( x )" := (Morph (x )) (in custom expr, x constr) : kappa_scope.
 
   Notation tupleHelper := (fun x y => App (App kappa_pair x) y).
   Notation "( x , .. , y , z )" := (
@@ -72,21 +72,21 @@ Module KappaNotation.
   Notation "'fst'" := (kappa_fst) (in custom expr at level 4) : kappa_scope.
   Notation "'snd'" := (kappa_snd) (in custom expr at level 4) : kappa_scope.
 
-  Notation "'not'" := (Morph not_gate) (in custom expr at level 4) : kappa_scope.
-  Notation "'and'" := (Morph and_gate) (in custom expr at level 4) : kappa_scope.
-  Notation "'nand'" := (Morph nand_gate) (in custom expr at level 4) : kappa_scope.
-  Notation "'or'" := (Morph or_gate) (in custom expr at level 4) : kappa_scope.
-  Notation "'nor'" := (Morph nor_gate) (in custom expr at level 4) : kappa_scope.
-  Notation "'xor'" := (Morph xor_gate) (in custom expr at level 4) : kappa_scope.
-  Notation "'xnor'" := (Morph xnor_gate) (in custom expr at level 4) : kappa_scope.
-  Notation "'buf'" := (Morph buf_gate) (in custom expr at level 4) : kappa_scope.
-  Notation "'delay'" := (Morph delay_gate) (in custom expr at level 4) : kappa_scope.
+  Notation "'not'" := (Morph (Primitive not_gate)) (in custom expr at level 4) : kappa_scope.
+  Notation "'and'" := (Morph (Primitive and_gate)) (in custom expr at level 4) : kappa_scope.
+  Notation "'nand'" := (Morph (Primitive nand_gate)) (in custom expr at level 4) : kappa_scope.
+  Notation "'or'" := (Morph (Primitive or_gate)) (in custom expr at level 4) : kappa_scope.
+  Notation "'nor'" := (Morph (Primitive nor_gate)) (in custom expr at level 4) : kappa_scope.
+  Notation "'xor'" := (Morph (Primitive xor_gate)) (in custom expr at level 4) : kappa_scope.
+  Notation "'xnor'" := (Morph (Primitive xnor_gate)) (in custom expr at level 4) : kappa_scope.
+  Notation "'buf'" := (Morph (Primitive buf_gate)) (in custom expr at level 4) : kappa_scope.
+  Notation "'delay'" := (Morph (Primitive delay_gate)) (in custom expr at level 4) : kappa_scope.
 
-  Notation "'xorcy'" := (Morph xorcy) (in custom expr at level 4) : kappa_scope.
-  Notation "'muxcy'" := (Morph muxcy) (in custom expr at level 4) : kappa_scope.
+  Notation "'xorcy'" := (Morph (Primitive xorcy)) (in custom expr at level 4) : kappa_scope.
+  Notation "'muxcy'" := (Morph (Primitive muxcy)) (in custom expr at level 4) : kappa_scope.
 
-  Definition unsigned_add2 {cava:Cava} {a b} := unsigned_add a b (S (max a b)).
-  Definition unsigned_add1 {cava:Cava} {a b} := unsigned_add a b (max a b).
+  Definition unsigned_add2 {a b} := Primitive (unsigned_add a b (S (max a b))).
+  Definition unsigned_add1 {a b} := Primitive (unsigned_add a b (max a b)).
 
   (* Notation "x + y" := (App (App (Morph (UnsignedAdd2 _ _)) x) y) (in custom expr at level 4) : kappa_scope. *)
   Notation "x + y" := 
@@ -95,56 +95,57 @@ Module KappaNotation.
   Notation "x +% y" := 
       (App (App (Morph unsigned_add1) x) y) 
       (in custom expr at level 4) : kappa_scope.
-  Notation "x - y" := (App (App (Morph (unsigned_sub _)) x) y) (in custom expr at level 4) : kappa_scope.
-  Notation "'unsigned_add' a b c" := (Morph (unsigned_add a b c))
+  Notation "x - y" := (App (App (Morph (Primitive (unsigned_sub _))) x) y) (in custom expr at level 4) : kappa_scope.
+  Notation "'unsigned_add' a b c" := (Morph (Primitive (unsigned_add a b c)))
     (in custom expr at level 4,
     a constr at level 4,
     b constr at level 4,
     c constr at level 4
     ) : kappa_scope.
-  Notation "'unsigned_sub' a" := (Morph (unsigned_sub a))
+  Notation "'unsigned_sub' a" := (Morph (Primitive (unsigned_sub a)))
     (in custom expr at level 4,
     a constr at level 4
     ) : kappa_scope.
 
-  Notation "'[]'" := (Morph (empty_vec _)) (in custom expr at level 4) : kappa_scope.
-  Notation "x ++ y" := (App (App (Morph (concat _ _)) x) y) (in custom expr at level 4) : kappa_scope.
-  Notation "x :: y" := (App (App (Morph (cons _ _)) x) y) (in custom expr at level 7, right associativity) : kappa_scope.
+  Notation "'[]'" := (Morph (Primitive (empty_vec _))) (in custom expr at level 4) : kappa_scope.
+  Notation "x ++ y" := (App (App (Morph (Primitive (concat _ _))) x) y) (in custom expr at level 4) : kappa_scope.
+  Notation "x :: y" := (App (App (Morph (Primitive (cons _ _))) x) y) (in custom expr at level 7, right associativity) : kappa_scope.
 
-  Notation "'true'" := (Morph (constant true)) (in custom expr at level 2) : kappa_scope.
-  Notation "'false'" := (Morph (constant false)) (in custom expr at level 2) : kappa_scope.
+  Notation "'true'" := (Morph (Primitive (constant true))) (in custom expr at level 2) : kappa_scope.
+  Notation "'false'" := (Morph (Primitive (constant false))) (in custom expr at level 2) : kappa_scope.
 
-  Notation "# x" := (Morph (constant_bitvec _ x))%N (in custom expr at level 2, x constr at level 4) : kappa_scope.
+  Notation "# x" := (Morph (Primitive (constant_bitvec _ x)))%N (in custom expr at level 2, x constr at level 4) : kappa_scope.
 
-  Notation "v [ x ]" := (App (App (Morph (index _ _)) v) x)
+  Notation "v [ x ]" := (App (App (Morph (Primitive (index _ _))) v) x)
     ( in custom expr at level 2
     , x at level 7
     ) : kappa_scope.
   Notation "v [: x : y ]" :=
-        (App (Morph (slice _ (x <: nat) (y <: nat) _ _ _)) v)
+        (App (Morph (Primitive (slice _ (x <: nat) (y <: nat) _))) v)
     (in custom expr at level 2,
     (* v constr, *)
     x constr at level 7,
     y constr at level 7
     ) : kappa_scope.
 
-  Notation "'index'" := (Morph (index _ _)) (in custom expr at level 4) : kappa_scope.
-  Notation "'empty'" := (Morph empty_vec) (in custom expr at level 4) : kappa_scope.
-  Notation "'cons'" := (Morph (cons _ _)) (in custom expr at level 4) : kappa_scope.
-  Notation "'snoc'" := (Morph (snoc _ _)) (in custom expr at level 4) : kappa_scope.
-  Notation "'concat'" := (Morph (concat _ _ _)) (in custom expr at level 4) : kappa_scope.
-  Notation "'split_at' x" := (Morph (split x _ _)) (in custom expr at level 4, x constr at level 4) : kappa_scope.
-  Notation "'uncons'" := (Morph (uncons _ _)) (in custom expr at level 4) : kappa_scope.
-  Notation "'unsnoc'" := (Morph (unsnoc _ _)) (in custom expr at level 4) : kappa_scope.
+  Notation "'index'" := (Morph (Primitive (index _ _))) (in custom expr at level 4) : kappa_scope.
+  Notation "'empty'" := (Morph (Primitive (empty_vec))) (in custom expr at level 4) : kappa_scope.
+  Notation "'cons'" := (Morph (Primitive (cons _ _))) (in custom expr at level 4) : kappa_scope.
+  Notation "'snoc'" := (Morph (Primitive (snoc _ _))) (in custom expr at level 4) : kappa_scope.
+  Notation "'concat'" := (Morph (Primitive (concat _ _ _))) (in custom expr at level 4) : kappa_scope.
+  Notation "'split_at' x" := (Morph (Primitive (split x _ _))) (in custom expr at level 4, x constr at level 4) : kappa_scope.
+  Notation "'uncons'" := (Morph (Primitive (uncons _ _))) (in custom expr at level 4) : kappa_scope.
+  Notation "'unsnoc'" := (Morph (Primitive (unsnoc _ _))) (in custom expr at level 4) : kappa_scope.
 
 
 End KappaNotation.
 
 Definition make_module {i o}
   (name: string)
-  (expr: forall cava: Cava, i ~[cava]~> o)
-  : forall cava: Cava, i ~[cava]~> o
-  := fun cava => mk_module _ _ name (expr _).
+  (expr: i ~> o)
+  : i ~> o
+  := expr.
+  (* mk_module _ _ name (expr _). *)
 
 Import KappaNotation.
 Local Open Scope kind_scope.
@@ -153,44 +154,43 @@ Section regression_examples.
   Import KappaNotation.
   Local Open Scope kappa_scope.
 
-  Program Definition ex0_constant: forall cava: Cava, << Vector Bit 10, Unit >> ~> (Vector Bit 8)
+  Definition ex0_constant:  << Vector Bit 10, Unit >> ~> (Vector Bit 8)
     := <[ \x => x [: 7 : 0 ] ]>.
-  Next Obligation. lia. Qed.
 
-  Definition ex1_constant: forall cava: Cava, << Bit, Unit >> ~> Bit := <[ \x => true ]>.
-  Definition ex2_parameterized (n: nat): forall cava: Cava, << Bit, Unit >> ~> Bit :=
+  Definition ex1_constant:  << Bit, Unit >> ~> Bit := <[ \x => true ]>.
+  Definition ex2_parameterized (n: nat):  << Bit, Unit >> ~> Bit :=
   match n with
   | O => <[ \ x => true ]>
   | S n => <[ \ x => xor x x ]>
   end.
 
-  Definition ex3_to_vec: forall cava: Cava, << Bit, Unit >> ~> (Vector Bit 1) :=
+  Definition ex3_to_vec:  << Bit, Unit >> ~> (Vector Bit 1) :=
   <[ \ x => x :: [] ]>.
-  Definition ex4_index_vec: forall cava: Cava, << Vector Bit 10, Unit >> ~> Bit :=
+  Definition ex4_index_vec:  << Vector Bit 10, Unit >> ~> Bit :=
   <[ \ x => index x (# 1) ]>.
-  Definition ex5_index_vec2: forall cava: Cava, << Vector Bit 10, Unit >> ~> Bit :=
+  Definition ex5_index_vec2:  << Vector Bit 10, Unit >> ~> Bit :=
   <[ \ x => x [# 1] ]>.
-  Definition ex6_concat: forall cava: Cava, << Vector Bit 2, Bit, Unit >> ~> (Vector Bit 3) :=
+  Definition ex6_concat:  << Vector Bit 2, Bit, Unit >> ~> (Vector Bit 3) :=
   <[ \ x v => snoc x v ]>.
-  Definition ex7_xor: forall cava: Cava, << Bit, Bit, Unit >> ~> Bit :=
+  Definition ex7_xor:  << Bit, Bit, Unit >> ~> Bit :=
   <[ \ x y => xor x y ]>.
-  Definition ex7_tupled_destruct: forall cava: Cava, << << Bit, Bit>>, Unit>> ~> Bit :=
+  Definition ex7_tupled_destruct:  << << Bit, Bit>>, Unit>> ~> Bit :=
   <[ \ xy =>
     let '(x,y) = xy in
     y ]>.
-  Definition ex8_multiindex: forall cava: Cava, << Vector (Vector Bit 5) 10, Unit >> ~> Bit :=
+  Definition ex8_multiindex:  << Vector (Vector Bit 5) 10, Unit >> ~> Bit :=
   <[ \ x => x[#0][#1] ]>.
-  Definition ex9_mkvec: forall cava: Cava, << Bit, Unit >> ~> (Vector Bit 2) :=
+  Definition ex9_mkvec:  << Bit, Unit >> ~> (Vector Bit 2) :=
   <[ \x => true :: false :: [] ]>.
-  Definition ex10: forall cava: Cava, << Vector Bit 10, Vector Bit 10, Unit >> ~> (Vector Bit 11) :=
+  Definition ex10:  << Vector Bit 10, Vector Bit 10, Unit >> ~> (Vector Bit 11) :=
   <[ \ x y => x + y ]>.
-  Definition ex11: forall cava: Cava, << Vector Bit 10, Vector Bit 10, Unit >> ~> (Vector Bit 10) :=
+  Definition ex11:  << Vector Bit 10, Vector Bit 10, Unit >> ~> (Vector Bit 10) :=
   <[ \ x y => x +% y ]>.
-  Definition ex12_module: forall cava: Cava, <<Vector Bit 10, Unit>> ~> Vector Bit 10
+  Definition ex12_module:  <<Vector Bit 10, Unit>> ~> Vector Bit 10
     := make_module "ex12_module" <[ \x => x +% x ]>.
-  Definition ex13: forall cava: Cava, << Vector Bit 10, Unit >> ~> Bit :=
+  Definition ex13:  << Vector Bit 10, Unit >> ~> Bit :=
   <[ \ x => (xor x[#0] x[#1] :: false :: []) [#0] ]>.
-  Definition ex14: forall cava: Cava, << Vector Bit 10, Vector Bit 4, Unit >> ~> Bit :=
+  Definition ex14:  << Vector Bit 10, Vector Bit 4, Unit >> ~> Bit :=
   <[ \ x i => x [ i ] ]>.
 
   Fixpoint copy_object_pow2 o (n:nat): Kind :=
@@ -202,9 +202,9 @@ Section regression_examples.
   Fixpoint tree
     (A: Kind)
     (n: nat)
-    (f: forall (cava: Cava), << A, A, Unit >> ~[cava]~> A)
+    (f: << A, A, Unit >> ~> A)
     {struct n}
-    : forall cava: Cava, << copy_object_pow2 A n, Unit >> ~> A :=
+    :  << copy_object_pow2 A n, Unit >> ~> A :=
   match n with
   | O => <[ \ x => x ]>
   | S n' =>
@@ -216,20 +216,20 @@ Section regression_examples.
   end.
 
   Definition add' (n: nat)
-    : forall cava: Cava, <<Vector Bit n, Vector Bit n, Unit>> ~> (Vector Bit n)
+    :  <<Vector Bit n, Vector Bit n, Unit>> ~> (Vector Bit n)
     :=
     match Nat.eq_dec (Init.Nat.max n n) n with
-    | left Heq => rew [fun x => forall cava: Cava, _~>Vector Bit x] Heq in <[\x y=> x +% y]>
+    | left Heq => rew [fun x =>  _~>Vector Bit x] Heq in <[\x y=> x +% y]>
     | right Hneq => (ltac:(lia))
     end.
 
   Definition adder_tree
     (bitsize n: nat)
-    : forall cava:Cava, <<copy_object_pow2 (Vector Bit bitsize) n, Unit>> ~> (Vector Bit bitsize) :=
+    : <<copy_object_pow2 (Vector Bit bitsize) n, Unit>> ~> (Vector Bit bitsize) :=
     tree (Vector Bit bitsize) n (add' bitsize).
 
   Definition xilinxFullAdder
-    : forall cava: Cava, << Bit, << Bit, Bit >>, Unit>> ~> (Tuple Bit Bit) :=
+    :  << Bit, << Bit, Bit >>, Unit>> ~> (Tuple Bit Bit) :=
     <[ \ cin ab =>
       let a = fst ab in
       let b = snd ab in
