cava/cava/Cava/Extraction.v
@@ -57,8 +57,8 @@ Recursive Extraction Library CavaArrow.
 Recursive Extraction Library CavaExpression.
 Recursive Extraction Library CavaNotation.
 Recursive Extraction Library CombinationalArrow.
-Recursive Extraction Library EvaluationArrow.
-Recursive Extraction Library NetlistArrow.
+(* Recursive Extraction Library EvaluationArrow. *)
+(* Recursive Extraction Library NetlistArrow. *)
 Recursive Extraction Library PropArrow.
 
 Recursive Extraction Library Netlist.
